cedar-lean/Cedar/Thm/Validation/RequestEntityValidation.lean
@@ -15,13 +15,14 @@ theorem instance_of_bool_type_refl (b : Bool) (bty : BoolType) :
   intro h₀
   cases h₁ : b <;> cases h₂ : bty <;> subst h₁ <;> subst h₂ <;> simp only [Bool.false_eq_true] at *
 
-theorem instance_of_entity_type_refl (e : EntityUID) (ety : EntityType) :
-  instanceOfEntityType e ety = true → InstanceOfEntityType e ety
+theorem instance_of_entity_type_refl (e : EntityUID) (ety : EntityType) (env : Environment) :
+  instanceOfEntityType e ety env = true → InstanceOfEntityType e ety env
 := by
   simp only [InstanceOfEntityType, instanceOfEntityType]
   intro h₀
-  simp only [beq_iff_eq] at h₀
-  assumption
+  simp at h₀
+  simp
+  exact h₀
 
 theorem instance_of_ext_type_refl (ext : Ext) (extty : ExtType) :
   instanceOfExtType ext extty = true → InstanceOfExtType ext extty
@@ -30,8 +31,8 @@ theorem instance_of_ext_type_refl (ext : Ext) (extty : ExtType) :
   intro h₀
   cases h₁ : ext <;> cases h₂ : extty <;> subst h₁ <;> subst h₂ <;> simp only [Bool.false_eq_true] at *
 
-theorem instance_of_type_refl (v : Value) (ty : CedarType) :
-  instanceOfType v ty = true → InstanceOfType v ty
+theorem instance_of_type_refl (v : Value) (ty : CedarType) (env : Environment) :
+  instanceOfType v ty env = true → InstanceOfType v ty
 := by
   intro h₀
   unfold instanceOfType at h₀
@@ -75,7 +76,7 @@ theorem instance_of_type_refl (v : Value) (ty : CedarType) :
       simp only [← Set.in_list_iff_in_set] at hv
       specialize h₀ ⟨v, hv⟩
       simp only [List.attach_def, List.mem_pmap_subtype, hv, true_implies] at h₀
-      exact instance_of_type_refl v sty h₀
+      exact instance_of_type_refl v sty env h₀
     all_goals
       contradiction
     all_goals
@@ -114,7 +115,7 @@ theorem instance_of_type_refl (v : Value) (ty : CedarType) :
         simp only [h₈] at h₇
         simp only [h₈, Option.some.injEq] at h₂
         subst h₂
-        exact instance_of_type_refl v vl.getType h₇
+        exact instance_of_type_refl v vl.getType env h₇
       intro k qty h₁ h₂
       have ⟨⟨_, h₄⟩, h₅⟩ := h₀
       clear h₀
@@ -158,13 +159,13 @@ decreasing_by
     have := Map.sizeOf_lt_of_value h₁
     omega
 
-theorem instance_of_request_type_refl (request : Request) (reqty : RequestType) :
-  instanceOfRequestType request reqty = true → InstanceOfRequestType request reqty
+theorem instance_of_request_type_refl (request : Request) (env : Environment) :
+  instanceOfRequestType request env = true → InstanceOfRequestType request env
 := by
   intro h₀
   simp only [InstanceOfRequestType]
   simp only [instanceOfRequestType, Bool.and_eq_true, beq_iff_eq] at h₀
-  obtain ⟨⟨⟨h₁,h₂⟩,h₃⟩, h₄⟩ := h₀
+  obtain ⟨⟨⟨⟨ h₁,h₂⟩,h₃⟩, h₄⟩, hₐ⟩ := h₀
   constructor
   case left =>
     apply instance_of_entity_type_refl
@@ -179,16 +180,20 @@ theorem instance_of_request_type_refl (request : Request) (reqty : RequestType) 
         apply instance_of_entity_type_refl
         exact h₃
       case right =>
-        apply instance_of_type_refl
-        exact h₄
+        constructor
+        case left =>
+          apply instance_of_type_refl
+          exact h₄
+        case right =>
+          apply instance_of_entity_type_refl _ _ _ hₐ
 
-theorem instance_of_entity_schema_refl (entities : Entities) (ets : EntitySchema) :
-  instanceOfEntitySchema entities ets = .ok () → InstanceOfEntitySchema entities ets
+theorem instance_of_entity_schema_refl (entities : Entities) (env : Environment) :
+  instanceOfEntitySchema entities env = .ok () → InstanceOfEntitySchema entities env.ets
 := by
   intro h₀
   simp only [InstanceOfEntitySchema]
   simp only [instanceOfEntitySchema] at h₀
-  generalize h₁ : (fun x : EntityUID × EntityData => instanceOfEntitySchema.instanceOfEntityData ets x.fst x.snd) = f
+  generalize h₁ : (fun x : EntityUID × EntityData => instanceOfEntitySchema.instanceOfEntityData env x.fst x.snd) = f
   rw [h₁] at h₀
   intro uid data h₂
   have h₀ := List.forM_ok_implies_all_ok (Map.toList entities) f h₀
@@ -196,14 +201,14 @@ theorem instance_of_entity_schema_refl (entities : Entities) (ets : EntitySchema
   have h₀ := h₀ (Map.find?_mem_toList h₂)
   rw [← h₁] at h₀
   simp only [instanceOfEntitySchema.instanceOfEntityData] at h₀
-  cases h₂ : Map.find? ets uid.ty <;> simp [h₂] at h₀
+  cases h₂ : Map.find? env.ets uid.ty <;> simp [h₂] at h₀
   case some entry =>
     exists entry
     simp only [true_and]
     split at h₀ <;> try simp only [reduceCtorEq] at h₀
     rename_i h₃
     constructor
-    · exact instance_of_type_refl (Value.record data.attrs) (CedarType.record entry.attrs) h₃
+    · exact instance_of_type_refl (Value.record data.attrs) (CedarType.record entry.attrs) env h₃
     · split at h₀ <;> try simp only [reduceCtorEq] at h₀
       rename_i h₄
       simp only [Set.all, List.all_eq_true] at h₄
@@ -257,10 +262,10 @@ theorem request_and_entities_match_env (env : Environment) (request : Request) (
   simp only [requestMatchesEnvironment] at h₀
   simp only [entitiesMatchEnvironment] at h₁
   constructor
-  exact instance_of_request_type_refl request env.reqty h₀
-  cases h₂ : instanceOfEntitySchema entities env.ets <;> simp only [h₂, Except.bind_err, Except.bind_ok, reduceCtorEq] at h₁
+  exact instance_of_request_type_refl request env h₀
+  cases h₂ : instanceOfEntitySchema entities env <;> simp only [h₂, Except.bind_err, Except.bind_ok, reduceCtorEq] at h₁
   constructor
-  exact instance_of_entity_schema_refl entities env.ets h₂
+  exact instance_of_entity_schema_refl entities env h₂
   exact instance_of_action_schema_refl entities env.acts h₁
 
 theorem request_and_entities_validate_implies_match_schema (schema : Schema) (request : Request) (entities : Entities) :
